Large checkpoint

examples/containers/proofs/IntSetPropertyProofs.v
@@ -1,234 +1,88 @@
+(******************************************************************************)
+(** Imports **)
+
+(* SSReflect *)
 From mathcomp Require Import ssreflect ssrbool ssrnat ssrfun seq eqtype.
 Set Bullet Behavior "Strict Subproofs".
 
+(* Basic Haskell libraries *)
 Require Import GHC.Base      Proofs.GHC.Base.
-Require Import Data.OldList  Proofs.Data.OldList.
+Require Import GHC.List      Proofs.GHC.List.
 Require Import Data.Foldable Proofs.Data.Foldable.
-Notation list := Coq.Init.Datatypes.list.
-Notation seq  := Coq.Lists.List.seq.
+Require Import Data.OldList  Proofs.Data.OldList.
+Require Import Data.Bits.
 
-Infix "=="  := op_zeze__ : bool_scope.
-Infix "===" := eq_op (at level 70, no associativity) : bool_scope.
-
-Notation "x == y :> A"  := (op_zeze__ (x : A) (y : A)) : bool_scope.
-Notation "x === y :> A" := (eq_op     (x : A) (y : A)) (at level 70, y at next level, no associativity) : bool_scope.
-
-Notation reflect := ssrbool.reflect. (* Why do I need this? *)
-
-Require Import Sorting.Sorted.
-Notation sort := Data.OldList.sort.
-
+(* IntSet *)
 Require Import Data.IntSet.Internal.
 Require Import IntSetProperties.
 Require Import IntSetProofs.
-Module IntSetFSet := Foo.
 
-Arguments "$"          {_ _}     / _ _.
-Arguments id           {_}       / _.
-Arguments Datatypes.id {_}       / _.
-Arguments forAll       {_ _ _ _} / _.
-Arguments "∘"          {_ _}     _ _ _ /.
+(* Working with Haskell *)
+Require Import OrdTactic.
+Require Import HSUtil IntSetUtil SortedUtil.
+
+(******************************************************************************)
+(** Name dismabiguation -- copied from HSUtil **)
+
+Notation list    := Coq.Init.Datatypes.list.
+Notation seq     := Coq.Lists.List.seq.
+Notation reflect := ssrbool.reflect.
+
+(******************************************************************************)
+(** Theorems **)
+(** The quoted comments and the section headers are taken directly from
+    `intset-properties.hs`. **)
+
+(********************************************************************
+  Valid IntMaps
+********************************************************************)
 
 Theorem thm_Valid : toProp prop_Valid.
 Proof.
   rewrite /prop_Valid /forValidUnitTree /forValid /=; apply valid_correct.
 Qed.
 
-Lemma WF_Bin_children (p : Prefix) (m : Mask) (l r : IntSet) :
-  WF (Bin p m l r) -> WF l /\ WF r.
-Proof.
-  case=> fn;
-    inversion 1    as [|s bounds fn' desc];
-    subst s fn';
-    inversion desc as [|l' bounds_l fn_l r' bounds_r fn_r
-                        p' m' bounds' fn'
-                        desc_l desc_r is_pos sub_l sub_r def_p def_m spec_fn];
-    subst p' m' l' r' bounds' fn'.
-  split; [exists fn_l | exists fn_r]; eauto using DescSem.
-Qed.
-
-Corollary WF_Bin_left (p : Prefix) (m : Mask) (l r : IntSet) :
-  WF (Bin p m l r) -> WF l.
-Proof. by move=> /WF_Bin_children []. Qed.
-
-Corollary WF_Bin_right (p : Prefix) (m : Mask) (l r : IntSet) :
-  WF (Bin p m l r) -> WF r.
-Proof. by move=> /WF_Bin_children []. Qed.
-
-Fixpoint iterates (n : nat) {a} (f : a -> a) (z : a) : list a :=
-  match n with
-  | O    => nil
-  | S n' => z :: iterates n' f (f z)
-  end.
-
-Lemma eftInt_aux_fuel_case (x y : Int) (p : GHC.Enum.eftInt_aux_fuel x y) :
-  (exists (gt : (x >? y)%Z = true),                  p = @GHC.Enum.done x y gt) \/
-  (exists (p' : GHC.Enum.eftInt_aux_fuel (x+1)%Z y), p = @GHC.Enum.step x y p').
-Proof.
-  case: p => [x' y' gt | x' y' p'].
-  - by left; exists gt.
-  - by right; exists p'.
-Qed.
-
-Require Import Coq.Logic.Eqdep_dec.
-
-Theorem UIP_refl_dec {A : Type} (dec : forall x y : A, {x = y} + {x <> y}) (x : A) (p : x = x) : p = erefl.
-Proof. exact (UIP_dec dec p erefl). Qed.
-
-Require Import GHC.Num.
-
-Theorem eftInt_aux_iterates (from to : Int) p :
-  @GHC.Enum.eftInt_aux from to p = iterates (Z.to_nat (to - from + #1)) (fun x => x + #1) from.
-Proof.
-  move: to p.
-  elim: from => [| from IHfrom | from IHfrom].
-  - elim=> [| to IHto | to IHto].
-    + move=> p; move: (eftInt_aux_fuel_case _ _ p) => [[gt def_p] | [p' def_p]]; subst p.
-      * by contradict gt.
-      * admit.
-    + simpl.
-Admitted.
-
-Require Import GHC.Num.
-Theorem enumFromTo_Int_iterates (from to : Int) :
-  enumFromTo from to = iterates (Z.to_nat (to - from + #1)) (fun x => x + #1) from.
-Proof. apply eftInt_aux_iterates. Qed.
-
-Theorem thm_MaskPow2 : toProp prop_MaskPow2.
-Proof.
-  simpl; elim=> [p m l IHl r IHr | p m | ] WF_s //=.
-  apply/and3P; split.
-  - rewrite /powersOf2 enumFromTo_Int_iterates.
-    cbv -[Z.pow member fromList].
-
-    inversion WF_s; inversion H; inversion HD; subst.
-    rewrite /rMask.
-    destruct r0 as [r0_1 r0_2].
-    
-(*     rewrite /powersOf2 enumFromTo_Int_iterates. *)
-(*     cbv -[Zpow member fromList]. *)
-
-    
-(*     move: (WF_s) => /WF_Bin_children [/IHl Pl /IHr Pr]. *)
-(*     move: Pl Pr; rewrite /prop_MaskPow2. *)
-
-(* rewrite /powersOf2 enumFromTo_Int_iterates. *)
-(*     cbv -[Zpow member fromList]. *)
-    
-(*     simpl *)
-
-(*  /=. *)
-(*     replace (GHC.Enum.eftInt 0%Z 63%Z) with (eftInt 0%Z 63%Z) by admit. *)
-    
-
-(*     cbv -[member fromList flat_map Zpow]. *)
-
-(*     rewrite /Enum.eftInt_fuel. *)
-    
-(*   - apply IHl; move: WF_s; apply WF_Bin_left. *)
-(*   - apply IHr; move: WF_s; apply WF_Bin_right. *)
-Abort.
-
-Theorem thm_AscDescList : toProp prop_AscDescList.
-Proof.
-  rewrite /prop_AscDescList /= => xs _.
-  rewrite /fromList /foldl /Foldable__list /Data.Foldable.Foldable__list_foldl /foldl /=.
-  rewrite /toAscList /toDescList.
-  rewrite foldl_foldr; last admit.
-  rewrite /flip.
-  unfold "_==_", Eq_list => /=.
-  
-  elim: xs => [|x xs IH] //=.
-Abort.
-
-Theorem thm_DescList : toProp prop_DescList.
-Proof.
-Abort.
-
-Theorem thm_Diff : toProp prop_Diff.
-Proof.
-  rewrite /prop_Diff /= => xs POS_xs ys POS_ys.
-  
-  move: (fromList_WF   xs POS_xs)       => WF_xs.
-  move: (fromList_WF   ys POS_ys)       => WF_ys.
-  move: (difference_WF _ _ WF_xs WF_ys) => WF_diff.
-  
-  split=> /=; first by apply valid_correct.
-Abort.
+(********************************************************************
+  Construction validity
+********************************************************************)
 
 Theorem thm_EmptyValid : toProp prop_EmptyValid.
 Proof. done. Qed.
 
-Lemma WRONG : forall x : Z, exists x' : N, x = Z.of_N x'. Admitted.
-Lemma eqIntSetMemberP {s1 s2 : IntSet} :
-  WF s1 -> WF s2 ->
-  reflect (forall x, member x s1 == member x s2) (s1 == s2).
+Theorem thm_SingletonValid : toProp prop_SingletonValid.
 Proof.
-  move=> WF1 WF2.
-  set s1' := exist _ _ WF1; set s2' := exist _ _ WF2.
-  move: (IntSetFSet.equal_1 s1' s2') (IntSetFSet.equal_2 s1' s2').
-  rewrite /= /IntSetFSet.Equal /= /IntSetFSet.In_set => Equal_eq eq_Equal.
-  apply iff_reflect; split.
-  - move=> KEYS; apply Equal_eq=> n; apply eq_iff_eq_true.
-    move: KEYS; cbv -[member Z.of_N eqb is_true].
-    rewrite -eqb_true_iff; apply.
-  - move=> /eq_Equal KEYS x; move: (WRONG x) => [n def_x]; subst x.
-    move: (KEYS n); cbv -[member Z.of_N eqb iff].
-    case: (member _ s1); case: (member _ s2); tauto.
+  rewrite /prop_SingletonValid /= => x POS_x.
+  by apply valid_correct, singleton_WF.
 Qed.
 
-Theorem Sem_member (s : IntSet) :
-  WF s ->
-  Sem s (member ^~ s).
+Theorem thm_InsertIntoEmptyValid : toProp prop_InsertIntoEmptyValid.
 Proof.
-  move=> [f def_f].
-  apply Sem_change_f with f => //.
-  by move: (def_f) => /member_Sem.
+  rewrite /prop_InsertIntoEmptyValid /= => x POS.
+  by apply valid_correct, insert_WF.
 Qed.
 
-Ltac member_by_Sem SEM :=
-  repeat (move=> /Sem_member ? || move=> ?);
-  erewrite member_Sem;
-    last (eapply SEM; try eassumption; reflexivity);
-    reflexivity.
+(********************************************************************
+  Single, Member, Insert, Delete, Member, FromList
+********************************************************************)
 
-Lemma insert_member (x : Int) (s : IntSet) :
-  (0 <= x)%Z -> WF s ->
-  forall k, member k (insert x s) = (k == x) || member k s.
-Proof. member_by_Sem insert_Sem. Qed.
+Theorem thm_Single : toProp prop_Single.
+Proof. by rewrite /prop_Single /= => x POS_x; apply/Eq_eq. Qed.
 
-Lemma delete_member (x : Int) (s : IntSet) :
-  (0 <= x)%Z -> WF s ->
-  forall k, member k (delete x s) = (k /= x) && member k s.
-Proof. member_by_Sem delete_Sem. Qed.
-
-Lemma union_member (s1 s2 : IntSet) :
-  WF s1 -> WF s2 ->
-  forall k, member k (union s1 s2) = member k s1 || member k s2.
-Proof. member_by_Sem union_Sem. Qed.
-
-Lemma intersection_member (s1 s2 : IntSet) :
-  WF s1 -> WF s2 ->
-  forall k, member k (intersection s1 s2) = member k s1 && member k s2.
-Proof. member_by_Sem intersection_Sem. Qed.
-
-Lemma difference_member (s1 s2 : IntSet) :
-  WF s1 -> WF s2 ->
-  forall k, member k (difference s1 s2) = member k s1 && ~~ member k s2.
-Proof. member_by_Sem difference_Sem. Qed.
-
-Lemma singleton_member (x : Int) :
-  (0 <= x)%Z ->
-  forall k, member k (singleton x) = (k == x).
-Proof. member_by_Sem singleton_Sem. Qed.
-
-Lemma EqExact_cases {A} `{EqExact A} (x y : A) :
-  {x == y /\ x = y} + {x /= y /\ x <> y}.
+Theorem thm_Member : toProp prop_Member.
 Proof.
-  rewrite Neq_inv; case CMP: (x == y).
-  - by left; split=> //; apply/Eq_eq.
-  - by right; split=> //; move=> /Eq_eq; rewrite CMP.
+  rewrite /prop_Member /= => xs POS_xs n POS_n.
+  rewrite !Foldable_all_ssreflect; apply/allP => /= k.
+  by rewrite fromList_member // Eq_refl.
 Qed.
+
+Theorem thm_NotMember : toProp prop_NotMember.
+Proof.
+  rewrite /prop_NotMember /= => xs POS_xs n POS_n.
+  rewrite !Foldable_all_ssreflect; apply/allP => /= k.
+  by rewrite /notMember /notElem /= fromList_member // Eq_refl.
+Qed.
+
+(* SKIPPED: test_LookupSomething, prop_LookupLT, prop_LookupGT, prop_LookupLE, prop_LookupGE *)
 
 Theorem thm_InsertDelete : toProp prop_InsertDelete.
 Proof.
@@ -238,7 +92,7 @@ Proof.
   move: (delete_WF x _ WF_ins POS) => WF_res.
   case x_nin_s: (~~ member x s) => //=; split=> /=; first by apply valid_correct.
 
-  apply/eqIntSetMemberP => // k; apply/Eq_eq.
+  apply/eqIntSetMemberP => // k POS_k.
   rewrite delete_member // insert_member //.
   rewrite Eq_inv andb_orr andbN orFb.
   
@@ -246,188 +100,6 @@ Proof.
   - by rewrite Peq; move: x_nin_s => /negbTE->; rewrite andbF.
   - by rewrite Bneq andTb.
 Qed.
-
-Theorem empty_WF : WF empty.
-Proof. by exists xpred0; constructor. Qed.
-Hint Resolve empty_WF.
-
-Theorem thm_InsertIntoEmptyValid : toProp prop_InsertIntoEmptyValid.
-Proof.
-  rewrite /prop_InsertIntoEmptyValid /= => x POS.
-  by apply valid_correct, insert_WF.
-Qed.
-
-Hypothesis sorted_sort : forall {A} `{Ord A} (xs : list A),
-  StronglySorted _<=_ (sort xs).
-
-Theorem elem_by_In {A} `{EqExact A} (xs : list A) (x : A) :
-  reflect (In x xs) (elem_by _==_ x xs).
-Proof.
-  elim: xs => [|x' xs IH] /=; first by constructor.
-  apply iff_reflect; split;
-    try move=> /orP;
-    move=> [? | ?];
-    try apply/orP;
-    solve [by left; apply/Eq_eq | by right; apply/IH].
-Qed.
-
-Hypothesis nub_NoDup : forall {A} `{EqExact A} (xs : list A),
-  NoDup (nub xs).
-
-Theorem thm_Int : toProp prop_Int.
-Proof.
-  rewrite /prop_Int /= => xs POS_xs ys POS_ys.
-
-  move: (fromList_WF     xs POS_xs)       => WF_xs.
-  move: (fromList_WF     ys POS_ys)       => WF_ys.
-  move: (intersection_WF _ _ WF_xs WF_ys) => WF_both.
-
-  split=> /=; first by apply valid_correct.
-  apply/Eq_eq; fold toList.
-Abort.
-
-Lemma Foldable_and_all {F} `{Foldable F} : and (t := F) =1 all id.
-Proof. done. Qed.
-
-Lemma toList_member_has (s : IntSet) :
-  WF s ->
-  forall k, has (_==_ k) (toList s) = member k s.
-Proof.
-  move=> /Sem_member/toList_In SEM k.
-  case CONT: (member k s) (SEM k) => SEM_k.
-  - have: In k (toList s) by apply SEM_k. clear SEM_k.
-    elim: (toList s) => [|x xs IH] //= SEM_k.
-    case: SEM_k => [-> | IN].
-    + by rewrite Eq_refl orTb.
-    + by rewrite IH // orbT.
-  - have: ~ In k (toList s) by move=> /SEM_k. clear SEM_k=> SEM_k.
-    apply negbTE; apply /negP; contradict SEM_k.
-    elim: (toList s) SEM_k => [|x xs IH] //= SEM_k.
-    move: SEM_k => /orP [/Eq_eq -> | H]; [by left | by right; apply IH].
-Qed.
-
-Lemma Int_eqbP : Equality.axiom (_==_ : Int -> Int -> bool).
-Proof. exact Eq_eq. Qed.
-
-Canonical Int_eqMixin := EqMixin Int_eqbP.
-Canonical Int_eqType := Eval hnf in EqType Int Int_eqMixin.
-
-Lemma InP {A : eqType} (x : A) (xs : list A) :
-  reflect (In x xs) (x \in xs).
-Proof.
-  elim: xs => [|y ys IH] //=.
-  - by rewrite seq.in_nil; constructor.
-  - rewrite inE; case CMP: (x === y) => /=.
-    + by constructor; left; apply/eqP; rewrite eq_sym.
-    + apply/equivP; first exact IH.
-      split; first by right.
-      case=> // ?; subst.
-      by move: CMP; rewrite eq_refl.
-Qed.
-
-Lemma elemC {A} `{Eq_ A} (a x : A) (xs : list A) : elem a (x :: xs) = (a == x) || elem a xs.
-Proof. done. Qed.
-
-Lemma elemN {A} `{Eq_ A} (a : A) : elem a [::] = false.
-Proof. done. Qed.
-
-Lemma elemP {A} `{EqExact A} (x : A) (xs : list A) :
-  reflect (In x xs) (elem x xs).
-Proof.
-  elim: xs => [|y ys IH] //=; first by constructor.
-  rewrite elemC; case CMP: (x == y) => /=.
-  - by constructor; left; apply/Eq_eq; rewrite Eq_sym.
-  - apply/equivP; first exact IH.
-    split; first by right.
-    case=> // ?; subst.
-    by move: CMP; rewrite Eq_refl.
-Qed.
-
-Lemma eqType_EqExact {A : eqType} `{EqExact A} (x y : A) : (x === y) = (x == y).
-Proof. by case E: (x === y); case E': (x == y)=> //; move: E E' => /eqP ? /Eq_eq ?. Qed.
-
-Lemma EqExact_eqType {A : eqType} `{EqExact A} (x y : A) : (x == y) = (x === y).
-Proof. by rewrite eqType_EqExact. Qed.
-
-Lemma elem_in {A : eqType} `{EqExact A} (xs : list A) (a : A) :
-  elem a xs = (a \in xs).
-Proof. by elim: xs => [|x xs IH] //=; rewrite inE -IH eqType_EqExact. Qed.
-
-Lemma in_elem {A : eqType} `{EqExact A} (xs : list A) (a : A) :
-  a \in xs = elem a xs.
-Proof. symmetry; apply elem_in. Qed.
-
-Theorem Foldable_all_ssreflect {A} (p : A -> bool) (xs : list A) : all p xs = seq.all p xs.
-Proof. by rewrite Foldable_all_forallb. Qed.
-
-Lemma fromList_member (xs : list Int) :
-  Forall (fun x => 0 <= x)%Z xs ->
-  forall k, member k (fromList xs) = elem k xs.
-Proof.
-  move=> POS_xs k.
-  move: (fromList_Sem xs POS_xs) => [f [SEM DEF]].
-  erewrite member_Sem; last by eapply SEM.
-  move: (DEF k); case: (f k) => DEF_k.
-  all: by symmetry; apply/elemP/DEF_k.
-Qed.
-
-Lemma toList_member (s : IntSet) :
-  WF s ->
-  forall k, elem k (toList s) = member k s.
-Proof.
-  move=> /Sem_member/toList_In SEM k.
-  by case CONT: (member k s) (SEM k) => SEM_k; apply/elemP/SEM_k.
-Qed.
-
-Theorem Sem_Desc0 : forall s f, Sem s f -> exists r, Desc0 s r f.
-Proof.
-  apply Sem_ind => [f false_f | s r f Desc_srf].
-  - by exists (0%Z,0%N); apply Desc0Nil.
-  - by exists r; apply (Desc0NotNil s r f r f); rewrite // isSubrange_refl.
-Qed.
-
-Theorem thm_LeftRight : toProp prop_LeftRight.
-Proof.
-  rewrite /prop_LeftRight /= => -[p m l r | // | // ] WF_x; move: (WF_x) => /WF_Bin_children [WF_l WF_r].
-  rewrite !Foldable_and_all !Foldable_all_ssreflect !flat_map_cons_f;
-    apply/andP; split; apply/allP => /= b /mapP [] x; rewrite in_elem toList_member // => x_in {b}->.
-  - case: (WF_x) => [f /Sem_Desc0 [rng DESC0]].
-    inversion_clear DESC0 as [|s rng' f' rng_ f'_ DESC rng'_rng f_f'].
-    inversion DESC; subst.
-Abort.
-
-Require Import OrdTactic.
-
-Theorem Sort_eq {A : eqType} `{OrdLaws A} `{!EqExact A} (xs ys : list A) :
-  StronglySorted _<=_ xs ->
-  StronglySorted _<=_ ys ->
-  (xs == ys) = seq.all (fun a => a \in xs) ys && seq.all (fun b => b \in ys) xs.
-Proof.
-  elim: xs ys => [|x xs IH_xs] [|y ys] //=.
-  inversion_clear 1 as [|X1 X2 SS_xs FA_xs X3]; inversion_clear 1 as [|X1 X2 SS_ys FA_ys X3].
-  unfold "=="; rewrite /Eq_list /=; case CMP: (x == y).
-  - move: CMP => /Eq_eq ? /=; subst y.
-    replace (eqlist xs ys) with (xs == ys) by done; rewrite IH_xs //.
-    admit.
-  - 
-Admitted.
-
-Theorem thm_List : toProp prop_List.
-Proof.
-  rewrite /prop_List /=; rewrite -/toList => xs POS_xs.
-Abort.
-  
-
-Theorem thm_Member : toProp prop_Member.
-Proof.
-  rewrite /prop_Member /= => xs POS_xs n POS_n.
-  rewrite !Foldable_all_ssreflect; apply/allP => /= k.
-  by rewrite fromList_member // Eq_refl.
-Qed.
-
-Lemma elem_app {A} `{Eq_ A} (a : A) (xs ys : list A) :
-  elem a (xs ++ ys) = elem a xs || elem a ys.
-Proof. by elim: xs => [|x xs] //=; rewrite !elemC -orbA => ->. Qed.
 
 (* Cheating: manually forgetting POS constraint *)
 Theorem thm_MemberFromList : toProp prop_MemberFromList.
@@ -457,50 +129,9 @@ Proof.
       apply Z.abs_nonneg.
 Qed.      
 
-Theorem thm_NotMember : toProp prop_NotMember.
-Proof.
-  rewrite /prop_NotMember /= => xs POS_xs n POS_n.
-  rewrite !Foldable_all_ssreflect; apply/allP => /= k.
-  by rewrite /notMember /notElem /= fromList_member // Eq_refl.
-Qed.
-
-Theorem thm_Prefix : toProp prop_Prefix.
-Proof.
-Abort.
-
-Theorem thm_Single : toProp prop_Single.
-Proof. by rewrite /prop_Single /= => x POS_x; apply/Eq_eq. Qed.
-
-Theorem thm_SingletonValid : toProp prop_SingletonValid.
-Proof.
-  rewrite /prop_SingletonValid /= => x POS_x.
-  by apply valid_correct, singleton_WF.
-Qed.
-
-Theorem thm_UnionAssoc : toProp prop_UnionAssoc.
-Proof.
-  rewrite /prop_UnionAssoc /= => s1 WF1 s2 WF2 s3 WF3.
-  
-  move: (union_WF _ _ WF1  WF2)  => WF12.
-  move: (union_WF _ _ WF2  WF3)  => WF23.
-  move: (union_WF _ _ WF12 WF3)  => WF123.
-  move: (union_WF _ _ WF1  WF23) => WF123'.
-  
-  apply/eqIntSetMemberP => // k; apply/Eq_eq.
-  by rewrite !union_member // orbA.
-Qed.
-
-Theorem thm_UnionComm : toProp prop_UnionComm.
-Proof.
-Proof.
-  rewrite /prop_UnionComm /= => s1 WF1 s2 WF2.
-  
-  move: (union_WF _ _ WF1 WF2) => WF12.
-  move: (union_WF _ _ WF2 WF1) => WF21.
-  
-  apply/eqIntSetMemberP => // k; apply/Eq_eq.
-  by rewrite !union_member // orbC.
-Qed.
+(********************************************************************
+  Union, Difference and Intersection
+********************************************************************)
 
 Theorem thm_UnionInsert : toProp prop_UnionInsert.
 Proof.
@@ -512,63 +143,274 @@ Proof.
 
   split=> /=; first by apply valid_correct.
   
-  apply/eqIntSetMemberP => // k; apply/Eq_eq.
+  apply/eqIntSetMemberP => // k POS_k.
   by rewrite union_member // singleton_member // insert_member // orbC.
 Qed.
+
+Theorem thm_UnionAssoc : toProp prop_UnionAssoc.
+Proof.
+  rewrite /prop_UnionAssoc /= => s1 WF1 s2 WF2 s3 WF3.
+  
+  move: (union_WF _ _ WF1  WF2)  => WF12.
+  move: (union_WF _ _ WF2  WF3)  => WF23.
+  move: (union_WF _ _ WF12 WF3)  => WF123.
+  move: (union_WF _ _ WF1  WF23) => WF123'.
+  
+  apply/eqIntSetMemberP => // k POS_k.
+  by rewrite !union_member // orbA.
+Qed.
+
+Theorem thm_UnionComm : toProp prop_UnionComm.
+Proof.
+Proof.
+  rewrite /prop_UnionComm /= => s1 WF1 s2 WF2.
+  
+  move: (union_WF _ _ WF1 WF2) => WF12.
+  move: (union_WF _ _ WF2 WF1) => WF21.
+  
+  apply/eqIntSetMemberP => // k POS_k.
+  by rewrite !union_member // orbC.
+Qed.
+
+Theorem thm_Diff : toProp prop_Diff.
+Proof.
+  rewrite /prop_Diff /= => xs POS_xs ys POS_ys.
+  
+  move: (fromList_WF   xs POS_xs)       => WF_xs.
+  move: (fromList_WF   ys POS_ys)       => WF_ys.
+  move: (difference_WF _ _ WF_xs WF_ys) => WF_diff.
+  
+  split=> /=; first by apply valid_correct.
+Abort.
+
+Theorem thm_Int : toProp prop_Int.
+Proof.
+  rewrite /prop_Int /= => xs POS_xs ys POS_ys.
+
+  move: (fromList_WF     xs POS_xs)       => WF_xs.
+  move: (fromList_WF     ys POS_ys)       => WF_ys.
+  move: (intersection_WF _ _ WF_xs WF_ys) => WF_both.
+
+  split=> /=; first by apply valid_correct.
+  apply/Eq_eq; fold toList.
+  apply StronglySorted_Zlt_eq_In; [by apply to_List_sorted | | ].
+  
+Abort.
 
 Theorem thm_disjoint : toProp prop_disjoint.
 Proof.
   rewrite /prop_disjoint /= => s1 WF1 s2 WF2.
   
   move: (intersection_WF _ _ WF1 WF2) => WF12.
+
+  apply/Eq_eq.
   
-  elim: s1 WF1 WF12 => [p m l IHl r IHr | p b | ] WF1 WF12.
-  - 
+  elim: s1 s2 WF1 WF2 WF12 => [p1 m1 l1 IHl1 r1 IHr1 | p1 b1 |] s2 //.
+  - elim: s2 p1 m1 l1 IHl1 r1 IHr1 => [p2 m2 l2 IHl2 r2 IHr2 | p2 b2 |] //= p1 m1 l1 IHl1 r1 IHr1 WF1 WF2 WF12.
+    all: move: (WF1) => /WF_Bin_children [WFl1 WFr1].
+    + move: (WF2) => /WF_Bin_children [WFl2 WFr2].
+      rewrite disjoint_eq intersection_eq /=.
+      repeat match goal with |- context[if ?b then _ else _] => case b => //= end.
+      all: try by rewrite ?IHl1 ?IHr1 ?IHl2 ?IHr2 //=; apply intersection_WF.
+      rewrite IHl1 //=; last by apply intersection_WF.
+      rewrite IHr1 //=; last by apply intersection_WF.
+      rewrite /bin.
+      by case: (intersection l1 l2); case: (intersection r1 r2).
+    + rewrite disjoint_eq intersection_eq /=.
+      repeat match goal with |- context[if ?b then _ else _] => case b => //= end.
+      * admit.
+      * admit.
+  - elim: s2 p1 b1 => [p2 m2 l2 IHl2 r2 IHr2 | p2 b2 |] //= p1 b1 WF1 WF2 WF12.
+    + rewrite disjoint_eq intersection_eq /=.
+      repeat match goal with |- context[if ?b then _ else _] => case b => //= end.
+      * admit.
+      * admit.
+    + rewrite disjoint_eq intersection_eq /=.
+      rewrite /tip.
+      case: (p1 == p2) => //=.
+      case: (N.land b1 b2 == 0%N) => //=.
 Abort.
 
-Theorem thm_filter : toProp prop_filter.
+(********************************************************************
+  Lists
+********************************************************************)
+
+(* SKIPPED: prop_Ordered *)
+
+Theorem thm_List : toProp prop_List.
+Proof.
+  rewrite /prop_List /=; rewrite -/toList => xs POS_xs.
+Abort.
+
+Theorem thm_DescList : toProp prop_DescList.
+Proof.
+  rewrite /prop_DescList /= => xs POS_xs.
+  replace (toDescList (fromList xs)) with (reverse (toAscList (fromList xs)))
+    by by rewrite !hs_coq_reverse_rev toDescList_spec //; apply fromList_WF.
+  apply/Eq_eq; f_equal.
+  (* thm_List *)
+Abort.
+
+Theorem thm_AscDescList : toProp prop_AscDescList.
+Proof.
+  rewrite /prop_AscDescList /= => xs POS_xs.
+  rewrite /toAscList toDescList_spec; last by apply fromList_WF.
+  by rewrite hs_coq_reverse_rev rev_involutive Eq_refl.
+Qed.
+
+(* SKIPPED: prop_fromList *)
+
+(********************************************************************
+  Bin invariants
+********************************************************************)
+
+(* "Check the invariant that the mask is a power of 2." *)
+Theorem thm_MaskPow2 : toProp prop_MaskPow2.
+Proof.
+  simpl; elim=> [p m l IHl r IHr | p m | ] WF_s //=.
+  apply/and3P; split.
+  - rewrite /powersOf2 enumFromTo_Int_iterates.
+    cbv -[Z.pow member fromList].
+
+    inversion WF_s; inversion H; inversion HD; subst.
+    rewrite /rMask.
+    destruct r0 as [r0_1 r0_2].
+    
+    (*
+    rewrite /powersOf2 enumFromTo_Int_iterates.
+    cbv -[Zpow member fromList].
+
+    
+    move: (WF_s) => /WF_Bin_children [/IHl Pl /IHr Pr].
+    move: Pl Pr; rewrite /prop_MaskPow2.
+
+rewrite /powersOf2 enumFromTo_Int_iterates.
+    cbv -[Zpow member fromList].
+    
+    simpl
+
+ /=.
+    replace (GHC.Enum.eftInt 0%Z 63%Z) with (eftInt 0%Z 63%Z) by admit.
+    
+
+    cbv -[member fromList flat_map Zpow].
+
+    rewrite /Enum.eftInt_fuel.
+    
+  - apply IHl; move: WF_s; apply WF_Bin_left.
+  - apply IHr; move: WF_s; apply WF_Bin_right.
+  *)
+Abort.
+
+(* "Check that the prefix satisfies its invariant." *)
+Theorem thm_Prefix : toProp prop_Prefix.
 Proof.
 Abort.
 
-Theorem thm_foldL : toProp prop_foldL.
+(* "Check that the left elements don't have the mask bit set, and the right ones
+   do." *)
+Theorem thm_LeftRight : toProp prop_LeftRight.
 Proof.
+  rewrite /prop_LeftRight /= => -[p m l r | // | // ] WF_x; move: (WF_x) => /WF_Bin_children [WF_l WF_r].
+  rewrite !Foldable_and_all !Foldable_all_ssreflect !flat_map_cons_f;
+    apply/andP; split; apply/allP => /= b /mapP [] x; rewrite in_elem toList_member // => x_in {b}->.
+  - case: (WF_x) => [f /Sem_Desc0 [rng DESC0]].
+    inversion_clear DESC0 as [|s rng' f' rng_ f'_ DESC rng'_rng f_f'].
+    inversion DESC; subst.
 Abort.
 
-Theorem thm_foldL : toProp prop_foldL.
-Proof.
-Abort.
+(********************************************************************
+  IntSet operations are like Set operations
+********************************************************************)
 
-Theorem thm_foldR : toProp prop_foldR.
-Proof.
-Abort.
-
-Theorem thm_foldR : toProp prop_foldR.
-Proof.
-Abort.
-
+(* "Check that IntSet.isProperSubsetOf is the same as Set.isProperSubsetOf." *)
 Theorem thm_isProperSubsetOf : toProp prop_isProperSubsetOf.
 Proof.
 Abort.
 
+(* "In the above test, isProperSubsetOf almost always returns False (since a
+   random set is almost never a subset of another random set).  So this second
+   test checks the True case." *)
+Theorem thm_isProperSubsetOf2 : toProp prop_isProperSubsetOf2.
+Proof.
+  rewrite /prop_isProperSubsetOf2 /= => s1 WF1 s2 WF2.
+  move: (union_WF _ _ WF1 WF2) => WF12.
+  apply/Eq_eq/bool_eq_iff.
+  
+  rewrite isProperSubsetOf_member //; intuition.
+  apply/implyP=> k_in_s1.
+  by rewrite union_member // k_in_s1 orTb.
+Qed.
+
 Theorem thm_isSubsetOf : toProp prop_isSubsetOf.
 Proof.
+  rewrite /prop_isSubsetOf /= => s1 WF1 s2 WF2.
 Abort.
 
-Theorem thm_map : toProp prop_map.
+Theorem thm_isSubsetOf2 : toProp prop_isSubsetOf2.
 Proof.
-Abort.
+  rewrite /prop_isSubsetOf2 /= => s1 WF1 s2 WF2.
+  move: (union_WF _ _ WF1 WF2) => WF12.
+  rewrite isSubsetOf_member // => k.
+  rewrite union_member //.
+  by apply/implyP => ->.
+Qed.
+
+Theorem thm_size : toProp prop_size.
+Proof.
+  rewrite /prop_size /= => s WF_s.
+  rewrite size_spec //.
+  split=> /=.
+  - change @foldl' with @foldl; rewrite foldl_spec // -Zlength_correct.
+    apply/Eq_eq.
+    replace (Zlength (toList s)) with (Zlength (toList s) + 0%Z) by rewrite /= Z.add_0_r //.
+    move: 0%Z => /=; elim: (toList s) => [|x xs IH] //= z.
+    by rewrite Zlength_cons -IH Z.add_succ_comm.
+  - by rewrite hs_coq_length_list Zlength_correct Eq_refl.
+Qed.
+
+(* SKIPPED: prop_findMax, prop_findMin *)
 
 Theorem thm_ord : toProp prop_ord.
 Proof.
 Abort.
 
-Theorem thm_partition : toProp prop_partition.
-Proof.
-Abort.
+(* SKIPPED: prop_readShow *)
 
-Theorem thm_size : toProp prop_size.
+Theorem thm_foldR : toProp prop_foldR.
 Proof.
-Abort.
+  rewrite /prop_foldR /= => s WF_s.
+  by rewrite Eq_refl.
+Qed.
+
+Theorem thm_foldR' : toProp prop_foldR'.
+Proof.
+  rewrite /prop_foldR' /= => s WF_s.
+  by rewrite Eq_refl.
+Qed.
+
+Theorem thm_foldL : toProp prop_foldL.
+Proof.
+  rewrite /prop_foldL /= => s WF_s.
+  by rewrite foldl_spec // -hs_coq_foldl_base Eq_refl.
+Qed.
+
+Theorem thm_foldL' : toProp prop_foldL'.
+Proof.
+  rewrite /prop_foldL' /=; change @foldl' with @foldl; apply thm_foldL.
+Qed.
+
+Theorem thm_map : toProp prop_map.
+Proof.
+  rewrite /prop_map /map /= => s WF_s.
+  rewrite map_id.
+  have POS_s: Forall [eta Z.le 0] (toList s) by apply/Forall_forall; apply toList_In_nonneg.
+  apply/eqIntSetMemberP=> //; first by apply fromList_WF.
+  move=> k POS_k.
+  by rewrite fromList_member // toList_member // Eq_refl.
+Qed.
+
+(* SKIPPED: prop_maxView, prop_minView *)
 
 Theorem thm_split : toProp prop_split.
 Proof.
@@ -582,10 +424,42 @@ Theorem thm_splitRoot : toProp prop_splitRoot.
 Proof.
 Abort.
 
-Theorem thm_isSubsetOf : toProp prop_isSubsetOf.
+Theorem thm_partition : toProp prop_partition.
 Proof.
-Abort.
+  rewrite /prop_partition /= => s WF_s _ _.
+  rewrite partition_filter //.
+  
+  have WF_odd:   WF (filter GHC.Real.odd                 s) by apply filter_WF.
+  have WF_even:  WF (filter (fun k => ~~ GHC.Real.odd k) s) by apply filter_WF.
+  move: (union_WF _ _ WF_odd WF_even) => WF_union.
+  
+  rewrite !Foldable_all_ssreflect.
+  repeat (split=> /=); try by apply valid_correct.
+  - apply/allP=> /= k.
+    by rewrite in_elem toList_member // filter_member // => /andP[].
+  - apply/allP=> /= k.
+    rewrite in_elem toList_member // filter_member // => /andP[].
+    by rewrite /GHC.Real.odd negb_involutive.
+  - apply/eqIntSetMemberP=> // k POS_k.
+    rewrite union_member // !filter_member //.
+    by case: (member k s)=> //=; rewrite orb_negb_r.
+Qed.
 
-Theorem thm_isProperSubsetOf : toProp prop_isProperSubsetOf.
+Theorem thm_filter : toProp prop_filter.
 Proof.
-Abort.
+  rewrite /prop_filter /= => s WF_s _ _.
+  
+  have WF_odd:   WF (filter GHC.Real.odd                 s) by apply filter_WF.
+  have WF_even:  WF (filter GHC.Real.even                s) by apply filter_WF.
+  have WF_even': WF (filter (fun k => ~~ GHC.Real.odd k) s) by apply filter_WF.
+  move: (union_WF _ _ WF_odd WF_even) => WF_union.
+  
+  repeat (split=> /=); try by apply valid_correct.
+  rewrite partition_filter //.
+  apply/andP; split; first by apply Eq_refl.
+  apply/eqIntSetMemberP=> // k POS_k.
+  rewrite !filter_member //.
+  by rewrite /GHC.Real.odd negb_involutive.
+Qed.
+
+(* SKIPPED: prop_bitcount *)
