examples/containers/proofs/HSUtil.v
@@ -1,0 +1,208 @@
+(******************************************************************************)
+(** Imports **)
+
+(* SSReflect *)
+From mathcomp Require Import ssreflect ssrbool ssrnat ssrfun seq eqtype.
+Set Bullet Behavior "Strict Subproofs".
+
+(* Basic Haskell libraries *)
+Require Import GHC.Base      Proofs.GHC.Base.
+Require Import GHC.List      Proofs.GHC.List.
+Require Import GHC.Enum.
+Require Import Data.Foldable Proofs.Data.Foldable.
+Require Import Data.OldList  Proofs.Data.OldList.
+
+(* IntSet for non-IntSet theorems *)
+Require IntSetProofs.
+
+(******************************************************************************)
+(** Name dismabiguation -- MUST BE COPIED LOCALLY **)
+
+Notation list    := Coq.Init.Datatypes.list.
+Notation seq     := Coq.Lists.List.seq.
+Notation reflect := ssrbool.reflect.
+  (* Why do I need `reflect`?  What other `reflect` is in scope? *)
+
+(******************************************************************************)
+(** Notation disambiguation **)
+
+Infix "=="  := op_zeze__ : bool_scope.
+Infix "===" := eq_op (at level 70, no associativity) : bool_scope.
+
+Notation "x == y :> A"  := (op_zeze__ (x : A) (y : A)) : bool_scope.
+Notation "x === y :> A" := (eq_op     (x : A) (y : A)) (at level 70, y at next level, no associativity) : bool_scope.
+
+(******************************************************************************)
+(** Easier simplification **)
+
+Global Arguments "$"          {_ _}     / _ _.
+Global Arguments id           {_}       / _.
+Global Arguments Datatypes.id {_}       / _.
+Global Arguments "∘"          {_ _}     _ _ _ /.
+
+(******************************************************************************)
+(** bool **)
+
+Theorem bool_eq_iff (b1 b2 : bool) : b1 = b2 <-> (b1 <-> b2).
+Proof.
+  move: b1 b2 => [] [] //.
+  all: split; try solve[discriminate | case=> *; exfalso; auto].
+Qed.  
+
+(******************************************************************************)
+(** EqTypes **)
+
+(* EqType <-> EqExact translation *)
+
+Theorem eqType_EqExact {A : eqType} `{EqExact A} (x y : A) : (x === y) = (x == y).
+Proof. by case E: (x === y); case E': (x == y)=> //; move: E E' => /eqP ? /Eq_eq ?. Qed.
+
+Theorem EqExact_eqType {A : eqType} `{EqExact A} (x y : A) : (x == y) = (x === y).
+Proof. by rewrite eqType_EqExact. Qed.
+
+(* EqExact decidability *)
+
+Theorem EqExact_cases {A} `{EqExact A} (x y : A) :
+  {x == y /\ x = y} + {x /= y /\ x <> y}.
+Proof.
+  rewrite Neq_inv; case CMP: (x == y).
+  - by left; split=> //; apply/Eq_eq.
+  - by right; split=> //; move=> /Eq_eq; rewrite CMP.
+Qed.
+
+Corollary EqExact_dec {A} `{EqExact A} (x y : A) :
+  {x = y} + {x <> y}.
+Proof. generalize (EqExact_cases x y); tauto. Qed.
+
+(* Int is an EqType *)
+
+Lemma Int_eqbP : Equality.axiom (_==_ : Int -> Int -> bool).
+Proof. exact Eq_eq. Qed.
+
+Canonical Int_eqMixin := EqMixin Int_eqbP.
+Canonical Int_eqType := Eval hnf in EqType Int Int_eqMixin.
+
+(******************************************************************************)
+(** Foldable and lists **)
+
+Theorem Foldable_and_all {F} `{Foldable F} : and (t := F) =1 all id.
+Proof. done. Qed.
+
+Theorem Foldable_all_ssreflect {A} (p : A -> bool) (xs : list A) : all p xs = seq.all p xs.
+Proof. by rewrite IntSetProofs.Foldable_all_forallb. Qed.
+
+Theorem hs_coq_reverse_rev {A} (xs : list A) : reverse xs = rev xs.
+Proof.
+  rewrite /reverse.
+  replace (rev xs) with (rev xs ++ [::]) by rewrite app_nil_r //.
+  elim: xs [::] => [|x xs IH] //= acc.
+  by rewrite IH -app_assoc.
+Qed.
+
+(******************************************************************************)
+(** List membership (`elem`, `In`, `\in`) **)
+
+Theorem elem_in {A : eqType} `{EqExact A} (xs : list A) (a : A) :
+  elem a xs = (a \in xs).
+Proof. by elim: xs => [|x xs IH] //=; rewrite inE -IH eqType_EqExact. Qed.
+
+Theorem in_elem {A : eqType} `{EqExact A} (xs : list A) (a : A) :
+  a \in xs = elem a xs.
+Proof. symmetry; apply elem_in. Qed.
+
+Theorem elemN {A} `{Eq_ A} (a : A) : elem a [::] = false.
+Proof. done. Qed.
+
+Theorem elemC {A} `{Eq_ A} (a x : A) (xs : list A) : elem a (x :: xs) = (a == x) || elem a xs.
+Proof. done. Qed.
+
+Theorem elemP {A} `{EqExact A} (x : A) (xs : list A) :
+  reflect (In x xs) (elem x xs).
+Proof.
+  elim: xs => [|y ys IH] //=; first by constructor.
+  rewrite elemC; case CMP: (x == y) => /=.
+  - by constructor; left; apply/Eq_eq; rewrite Eq_sym.
+  - apply/equivP; first exact IH.
+    split; first by right.
+    case=> // ?; subst.
+    by move: CMP; rewrite Eq_refl.
+Qed.
+
+Theorem elem_app {A} `{Eq_ A} (a : A) (xs ys : list A) :
+  elem a (xs ++ ys) = elem a xs || elem a ys.
+Proof. by elim: xs => [|x xs] //=; rewrite !elemC -orbA => ->. Qed.
+
+Theorem elem_by_In {A} `{EqExact A} (xs : list A) (x : A) :
+  reflect (In x xs) (elem_by _==_ x xs).
+Proof.
+  elim: xs => [|x' xs IH] /=; first by constructor.
+  apply iff_reflect; split;
+    try move=> /orP;
+    move=> [? | ?];
+    try apply/orP;
+    solve [by left; apply/Eq_eq | by right; apply/IH].
+Qed.
+
+(* Non-Haskell theorems about In *)
+
+Theorem InP {A : eqType} (x : A) (xs : list A) :
+  reflect (In x xs) (x \in xs).
+Proof.
+  elim: xs => [|y ys IH] //=.
+  - by rewrite seq.in_nil; constructor.
+  - rewrite inE; case CMP: (x === y) => /=.
+    + by constructor; left; apply/eqP; rewrite eq_sym.
+    + apply/equivP; first exact IH.
+      split; first by right.
+      case=> // ?; subst.
+      by move: CMP; rewrite eq_refl.
+Qed.
+
+Theorem In_split {A} (x : A) (xs : list A) :
+  In x xs <->
+  exists pre post, xs = pre ++ x :: post.
+Proof.
+  split.
+  - elim: xs => [|x' xs IH] //= [? | IN]; first subst x'.
+    + by exists [::], xs.
+    + move: (IH IN) => [pre [post ->]].
+      by exists (x' :: pre), post.
+  - move=> [pre [post ->]].
+    by elim: pre => [|p pre IH] //=; [left | right].
+Qed.
+
+(******************************************************************************)
+(** Enum **)
+
+(* Missing function *)
+Fixpoint iterates (n : nat) {a} (f : a -> a) (z : a) : list a :=
+  match n with
+  | O    => nil
+  | S n' => z :: iterates n' f (f z)
+  end.
+
+Lemma eftInt_aux_fuel_case (x y : Int) (p : GHC.Enum.eftInt_aux_fuel x y) :
+  (exists (gt : (x >? y)%Z = true),                  p = @GHC.Enum.done x y gt) \/
+  (exists (p' : GHC.Enum.eftInt_aux_fuel (x+1)%Z y), p = @GHC.Enum.step x y p').
+Proof.
+  case: p => [x' y' gt | x' y' p'].
+  - by left; exists gt.
+  - by right; exists p'.
+Qed.
+
+Theorem eftInt_aux_iterates (from to : Int) p :
+  @GHC.Enum.eftInt_aux from to p = iterates (Z.to_nat (to - from + #1)) (fun x => x + #1) from.
+Proof.
+  move: to p.
+  elim: from => [| from IHfrom | from IHfrom].
+  - elim=> [| to IHto | to IHto].
+    + move=> p; move: (eftInt_aux_fuel_case _ _ p) => [[gt def_p] | [p' def_p]]; subst p.
+      * by contradict gt.
+      * admit.
+    + simpl.
+Admitted.
+
+Require Import GHC.Num.
+Theorem enumFromTo_Int_iterates (from to : Int) :
+  enumFromTo from to = iterates (Z.to_nat (to - from + #1)) (fun x => x + #1) from.
+Proof. apply eftInt_aux_iterates. Qed.
